template-coq/theories/AstUtils.v
@@ -180,7 +180,7 @@ Fixpoint remove_arity (n : nat) (t : term) : term :=
           end
   end.
 
-Fixpoint lookup_mind_decl (id : kername) (decls : global_env)
+Fixpoint lookup_mind_decl (id : kername) (decls : global_declarations)
  := match decls with
     | nil => None
     | (kn, InductiveDecl d) :: tl =>
@@ -190,8 +190,8 @@ Fixpoint lookup_mind_decl (id : kername) (decls : global_env)
 
 Definition universes_entry_of_decl (u : universes_decl) : universes_entry :=
   match u with
-  | Polymorphic_ctx ctx => Polymorphic_entry (fst ctx) (Universes.AUContext.repr ctx)
-  | Monomorphic_ctx ctx => Monomorphic_entry ctx
+  | Polymorphic_ctx ctx => Polymorphic_entry (Universes.AUContext.repr ctx)
+  | Monomorphic_ctx => Monomorphic_entry ContextSet.empty
   end.
 
 (* TODO factorize in Environment *)
